Progress

tests/lean/run/tailrec.lean
@@ -1,3 +1,17 @@
+def loop (x : Nat) : Unit := loop (x + 1)
+termination_by tailrecursion
+
+/--
+info: equations:
+theorem loop.eq_1 : ∀ (x : Nat), loop x = loop (x + 1)
+-/
+#guard_msgs in
+#print equations loop
+
+/-- error: unknown constant 'loop.induct' -/
+#guard_msgs in
+#check loop.induct
+
 def find (P : Nat → Bool) (x : Nat) : Option Nat :=
   if P x then
     some x
@@ -5,15 +19,72 @@ def find (P : Nat → Bool) (x : Nat) : Option Nat :=
     find P (x +1)
 termination_by tailrecursion
 
+/--
+info: equations:
+theorem find.eq_1 : ∀ (P : Nat → Bool) (x : Nat), find P x = if P x = true then some x else find P (x + 1)
+-/
+#guard_msgs in
 #print equations find
 
-
 /--
-error: failed to synthesize
-  Inhabited (Fin n)
-Additional diagnostic information may be available using the `set_option diagnostics true` command.
+error: Termination by tailrecursion needs an inhabited codomain:
+  failed to synthesize
+    Inhabited (Fin n)
+  Additional diagnostic information may be available using the `set_option diagnostics true` command.
 -/
 #guard_msgs in
 def notinhabited (n m : Nat) : Fin n :=
   notinhabited n (m+1)
 termination_by tailrecursion
+
+def fib (n : Nat) := go 0 0 1
+where
+  go i fip fi :=
+    if i = n then
+      fi
+    else
+      go (i + 1) fi (fi + fip)
+  termination_by tailrecursion
+
+/--
+error: fail to show termination for
+  mutual1
+  mutual2
+with errors
+failed to infer structural recursion:
+Cannot use parameters n of mutual1 and n of mutual2:
+  failed to eliminate recursive application
+    mutual2 (m + 1) n
+Cannot use parameters n of mutual1 and m of mutual2:
+  failed to eliminate recursive application
+    mutual2 (m + 1) n
+Cannot use parameters m of mutual1 and n of mutual2:
+  failed to eliminate recursive application
+    mutual2 (m + 1) n
+Cannot use parameters m of mutual1 and m of mutual2:
+  failed to eliminate recursive application
+    mutual2 (m + 1) n
+
+
+Could not find a decreasing measure.
+The arguments relate at each recursive call as follows:
+(<, ≤, =: relation proved, ? all proofs failed, _: no proof attempted)
+Call from mutual1 to mutual2 at 88:34-51:
+  n m
+n ? ?
+m = ?
+Call from mutual2 to mutual1 at 89:34-51:
+  n m
+n _ ?
+m _ _
+
+Please use `termination_by` to specify a decreasing measure.
+
+Termination by tailrecursion cannot handle dependent type:
+  (x : (_ : Nat) ×' Nat ⊕' (_ : Nat) ×' Nat) → PSum.casesOn x (fun _x => Unit) fun _x => Unit
+-/
+#guard_msgs in
+mutual
+def mutual1 (n m : Nat) : Unit := mutual2 (m + 1) n
+def mutual2 (n m : Nat) : Unit := mutual1 (m + 1) n
+end
